pass

src/Iris/Algebra/GenSet.lean
@@ -42,7 +42,9 @@ namespace GenSetDisj
 
 abbrev gen_set_valid : S → GenSetDisjO S := fun X => .mk (.set_valid X)
 
-variable {S : Type _} [LawfulSet S A]
+section dec_disj
+
+variable {S : Type _} [LawfulSet S A] [DecidableDisj S]
 
 def unit : GenSetDisjO S := gen_set_valid ∅
 
@@ -53,111 +55,46 @@ def valid (x : GenSetDisjO S) : Prop :=
   | .set_valid _ => True
   | _ => False
 
-theorem unit_valid : valid (unit (S := S)) := by simp [unit, valid]
-
 def validN : Nat → GenSetDisjO S → Prop := fun _ x => valid x
-
-theorem pcore_ne {x y : GenSetDisjO S} : x ≡{n}≡ y → pcore x = some cx →
-  ∃ cy, pcore y = some cy ∧ cx ≡{n}≡ cy := by
-  intro H1 H2
-  exists cx
-
-theorem validN_ne : x ≡{n}≡ y → validN n x → validN n y := by
-  intro H G; rw [<-H]; assumption
-
-theorem valid_iff_validN : valid x ↔ ∀ n, validN n x := by
-  apply Iff.intro
-  · intro H n; apply H
-  · intro H; apply H 0
-
-theorem validN_succ : validN n.succ x → validN n x := by
-  intro H; apply H
-
-theorem pcore_idem {x : GenSetDisjO S} : pcore x = some cx → pcore cx ≡ some cx := by
-  rcases x with ⟨x | _⟩ <;> rcases cx with ⟨cx | _⟩ <;> simp [pcore, unit]
-
-theorem pcore_unit : pcore (unit : GenSetDisjO S) ≡ some unit := by
-  simp [pcore, unit]
-
-variable [∀ X₁ X₂ : S, Decidable (X₁ ## X₂)]
 
 def op (x y : GenSetDisjO S) : GenSetDisjO S :=
   match x.car, y.car with
-  | .set_valid x, .set_valid y => if (x ## y) then .mk (.set_valid (x ∪ y)) else .mk .set_invalid
-  | _, _ => .mk .set_invalid
-
-theorem validN_op_left {x y : GenSetDisjO S} : validN n (op x y) → validN n x := by
-  rcases x, y with ⟨⟨⟨x⟩ | _⟩, ⟨⟨y⟩ | _⟩⟩ <;> simp [op, validN, valid]
+  | .set_valid x, .set_valid y => if (x ## y) then ⟨.set_valid (x ∪ y)⟩ else ⟨.set_invalid⟩
+  | _, _ => ⟨.set_invalid⟩
 
 instance op_ne {x : GenSetDisjO S} : OFE.NonExpansive (op x) where
-  ne n y z H := by rw [H]
+  ne _ _ _ H := by rw [H]
 
 theorem assoc {x y z : GenSetDisjO S} : op x (op y z) ≡ op (op x y) z := by
   rcases x, y, z with ⟨⟨⟨x⟩ | _⟩, ⟨⟨y⟩ | _⟩, ⟨⟨z⟩ | _⟩⟩ <;> simp [op]
-  if H : y ## z
-  then
-    simp [H]
-    if G : x ## y
-    then
-      simp [G]
-      if J : x ## z
-      then
-        have K1 : x ## y ∪ z := by
-          symm
-          rw [disjoint_union_left]; apply And.intro <;> (symm; assumption)
-        have K2 : x ∪ y ## z := by
-          rw [disjoint_union_left]; apply And.intro <;> assumption
-        simp [K1, K2]
-        rw [union_assoc]
-      else
-        have K1 : ¬ x ## y ∪ z := by
-          intro C
-          symm at C; rw [disjoint_union_left] at C
-          apply J; symm; exact C.right
-        have K2 : ¬ x ∪ y ## z := by
-          rw [disjoint_union_left, not_and]
-          intro C
-          exfalso; apply J C
-        simp [K1, K2]
-    else
-      simp [G]
+  by_cases H : y ## z
+  · simp only [H, ↓reduceIte]
+    by_cases G : x ## y
+    · simp [G, ↓reduceIte]
+      by_cases J : x ## z
+      · simp [↓reduceIte, union_assoc
+          , show x ## y ∪ z by
+              symm; rw [disjoint_union_left]; exact ⟨disjoint_symm G, disjoint_symm J⟩
+          , show x ∪ y ## z by rw [disjoint_union_left]; exact ⟨J, H⟩]
+      · simp [↓reduceIte
+          , show ¬ x ## y ∪ z by
+              intro C; rw [disjoint_comm, disjoint_union_left] at C; exact (J (disjoint_symm C.right))
+          , show ¬ x ∪ y ## z by
+              intro C; rw [disjoint_comm, disjoint_union_right] at C; exact (J (disjoint_symm C.left))]
+    · simp only [G, ↓reduceIte, ite_eq_right_iff, LeibnizO.mk.injEq, reduceCtorEq, imp_false]
       intro C; symm at C; rw [disjoint_union_left] at C
-      apply (G (disjoint_symm C.left))
-  else
-    simp [H]
-    if G : x ## y
-    then
-      simp [G]
-      intro C; apply H
-      rw [disjoint_union_left] at C
-      apply C.right
-    else
-      simp [G]
+      exact (G (disjoint_symm C.left))
+  · simp only [H, ↓reduceIte]
+    by_cases G : x ## y
+    · simp only [G, ↓reduceIte, right_eq_ite_iff, LeibnizO.mk.injEq, reduceCtorEq, imp_false]
+      intro C; rw [disjoint_union_left] at C; exact H C.right
+    · simp [G]
 
 theorem comm {x y : GenSetDisjO S} : op x y ≡ op y x := by
   rcases x, y with ⟨⟨⟨x⟩ | _⟩, ⟨⟨y⟩ | _⟩⟩ <;> simp [op]
-  if H : x ## y
-  then
-    have H' : y ## x := by symm; assumption
-    simp [H, H', union_comm]
-  else
-    simp [H]
-    intro c; apply H (disjoint_symm c)
-
-theorem pcore_op_left {x : GenSetDisjO S} : pcore x = some cx → op cx x ≡ x := by
-  rcases x with ⟨x | _⟩ <;> rcases cx with ⟨cx | _⟩ <;> simp [op, pcore, unit]
-  rintro ⟨⟩; simp [disjoint_empty_left]
-
-theorem pcore_op_mono {x : GenSetDisjO S} : pcore x = some cx → ∀ y, ∃ cy, pcore (op x y) ≡ some (op cx cy) := by
-  rcases x with ⟨x | _⟩ <;> simp only [pcore, Option.some.injEq, leibniz] <;> rintro ⟨⟩ y
-  <;> (exists unit; simp only [unit, op, disjoint_empty_left, ↓reduceIte, union_idem])
-
-def extend {x y₁ y₂ : GenSetDisjO S} (H : x ≡{n}≡ op y₁ y₂) :
-    Σ' z₁ z₂, x ≡ op z₁ z₂ ∧ z₁ ≡{n}≡ y₁ ∧ z₂ ≡{n}≡ y₂ := by
-  exists y₁, y₂
-
-theorem unit_left_id {x : GenSetDisjO S} : op unit x ≡ x := by
-  rcases x with ⟨x | _⟩ <;> simp [op, unit, disjoint_empty_left]
+  by_cases H : x ## y
+  · simp [H, union_comm, show y ## x by symm; assumption]
+  · simp [H]; intro c; exact H (disjoint_symm c)
 
 instance : CMRA (GenSetDisjO S) where
   pcore := pcore
@@ -165,70 +102,67 @@ instance : CMRA (GenSetDisjO S) where
   ValidN := validN
   Valid := valid
   op_ne := op_ne
-  pcore_ne := pcore_ne
-  validN_ne := validN_ne
-  valid_iff_validN := valid_iff_validN
-  validN_succ := validN_succ
-  validN_op_left := validN_op_left
+  pcore_ne {_ _ _ cx} _ H := ⟨cx, H, rfl⟩
+  validN_ne H G := H ▸ G
+  valid_iff_validN := ⟨(fun _ => ·), (· 0)⟩
+  validN_succ := id
+  validN_op_left {_ x y} := by rcases x, y with ⟨⟨⟨x⟩ | _⟩, ⟨⟨y⟩ | _⟩⟩ <;> simp [op, validN, valid]
   assoc := assoc
   comm := comm
-  pcore_op_left := pcore_op_left
-  pcore_idem := pcore_idem
-  pcore_op_mono := pcore_op_mono
-  extend _ := extend
+  pcore_op_left {cx x} := by
+    rcases x with ⟨x | _⟩ <;> rcases cx with ⟨cx | _⟩ <;> simp [op, pcore, unit]
+    rintro ⟨⟩; simp [disjoint_empty_left]
+  pcore_idem {x cx} := by rcases x with ⟨x | _⟩ <;> rcases cx with ⟨cx | _⟩ <;> simp [pcore, unit]
+  pcore_op_mono {_ x} := by
+    rcases x with ⟨x | _⟩ <;> simp only [pcore, Option.some.injEq, leibniz] <;> rintro ⟨⟩ y
+    <;> (exists unit; simp only [unit, op, disjoint_empty_left, ↓reduceIte, union_idem])
+  extend {_ _ y₁ y₂} _ h := ⟨y₁, y₂, ⟨h, rfl, rfl⟩⟩
 
 instance : CMRA.Discrete (GenSetDisjO S) where
-  discrete_valid := by intro x Hx; apply Hx
+  discrete_valid {_} := id
 
 instance : UCMRA (GenSetDisjO S) where
   unit := unit
-  unit_valid := unit_valid
-  unit_left_id := unit_left_id
-  pcore_unit := pcore_unit
+  unit_valid := by simp [unit, CMRA.Valid, valid]
+  unit_left_id {x} := by rcases x with ⟨x | _⟩ <;> simp [op, unit, disjoint_empty_left, CMRA.op]
+  pcore_unit := by simp [unit, CMRA.pcore, pcore]
 
 theorem set_disj_included (X Y : S) :
    gen_set_valid X ≼ gen_set_valid Y ↔ X ⊆ Y := by
   simp only [CMRA.Included]
-  apply Iff.intro
+  constructor
   · intro ⟨Z, HZ⟩
     rcases Z with ⟨Z | _⟩
-    · if H : X ## Z
-      then
-        simp [CMRA.op, op, H] at HZ; rw [HZ]
+    · by_cases H : X ## Z
+      · simp [CMRA.op, op, H] at HZ; rw [HZ]
         intro p Hp; rw [mem_union]; left; exact Hp
-      else
-        simp [CMRA.op, op, H] at HZ
+      · simp [CMRA.op, op, H] at HZ
     · simp [CMRA.op, op] at HZ
   · intro Hsub
     exists gen_set_valid (Y \ X)
-    have H : X ## (Y \ X) := by
-      intro p ⟨H1, H2⟩
-      rw [mem_diff] at H2
-      apply H2.right H1
-    simp [CMRA.op, op, H]
+    simp [CMRA.op, op, show X ## (Y \ X) by intro p ⟨H1, H2⟩; rw [mem_diff] at H2; exact H2.right H1]
     ext p; rw [mem_union, mem_diff]
-    apply Iff.intro
+    constructor
     · intro G
       by_cases H : (p ∈ X)
       · left; exact H
       · right; exact ⟨G, H⟩
     · rintro (G|G)
-      · apply Hsub _ G
-      · apply G.left
+      · exact Hsub _ G
+      · exact G.left
 
 theorem set_disj_union (X Y : S) (Hdisj : X ## Y) :
   (gen_set_valid X) • (gen_set_valid Y) ≡ gen_set_valid (X ∪ Y) := by
-  simp [CMRA.op, op]
-  exact Hdisj
+  simp only [CMRA.op, op, Hdisj, ↓reduceIte, gen_set_valid]; rfl
 
 theorem set_disj_valid_op (X Y : S) :
     ✓ ((gen_set_valid X) • (gen_set_valid Y)) ↔ X ## Y := by
-  simp [CMRA.op, op, CMRA.Valid, valid]
+  simp only [CMRA.op, op, CMRA.Valid, valid]
   by_cases H : X ## Y <;> simp [H]
 
 theorem set_disj_valid_inv_l (X : S) (Y : GenSetDisjO S) :
     ✓ ((gen_set_valid X) • Y) → ∃ Y', Y = gen_set_valid Y' ∧ X ## Y' := by
-  simp [CMRA.op, op, CMRA.Valid, valid]
+  simp only [CMRA.op, op, CMRA.Valid, valid]
   rcases Y with ⟨Y | _⟩ <;> simp <;> by_cases H : X ## Y <;> simp [H]
 
 theorem set_disj_dealloc_local_update (X Y : S) :
@@ -240,13 +174,16 @@ theorem set_disj_dealloc_local_update (X Y : S) :
   constructor
   · simp [CMRA.Valid, valid]
   · rcases z with ⟨z|_⟩
-    <;> simp [CMRA.op, op, disjoint_empty_left] at *
-    <;> if Hdisj : (Y ## z)
-        then simp [Hdisj] at heq; rw [heq]; ext i;
-             rw [mem_diff, mem_union];
-             specialize (Hdisj i);
-             grind only
-        else simp [Hdisj] at heq
+    · simp only [CMRA.op, op, leibniz, disjoint_empty_left, ↓reduceIte, union_empty_left,
+      LeibnizO.mk.injEq, set_valid.injEq] at heq ⊢
+      by_cases Hdisj : Y ## z <;> simp only [Hdisj, ↓reduceIte] at heq
+      · simp only [LeibnizO.mk.injEq, set_valid.injEq] at heq
+        ext i; rw [heq, mem_diff, mem_union]
+        specialize (Hdisj i)
+        grind
+      · cases heq
+    · simp only [CMRA.op, op, leibniz] at heq
+      cases heq
 
 theorem set_disj_dealloc_empty_local_update (X Z : S)  :
     (gen_set_valid Z • gen_set_valid X, gen_set_valid Z) ~l~>
@@ -261,7 +198,7 @@ theorem set_disj_dealloc_empty_local_update (X Z : S)  :
       · intro Hz; exact Hdisj a ⟨Hz, Ha⟩
     · intro ⟨Ha, Ha'⟩
       rcases Ha with Ha | Ha
-      · exfalso; exact Ha' Ha
+      · exact (Ha' Ha).elim
       · exact Ha
   rw [set_disj_union Z X Hdisj]
   conv => rhs; rw [Heq]
@@ -299,6 +236,8 @@ theorem set_disj_alloc_empty_local_update (X Z : S) (Hdisj : Z ## X) :
   rw [show gen_set_valid Z ≡ gen_set_valid (Z ∪ ∅) by simp [union_empty_right]]
   exact set_disj_alloc_local_update X ∅ Z Hdisj
 
+end dec_disj
+
 end GenSetDisj
 
 section Def
@@ -323,8 +262,6 @@ def pcore (x : GenSetO S) : Option (GenSetO S) := some x
 
 def valid (_x : GenSetO S) : Prop := True
 
-theorem unit_valid : valid (unit (S := S)) := by simp [valid]
-
 def validN (_n : Nat) (x : GenSetO S) : Prop := valid x
 
 theorem pcore_ne {x y : GenSetO S} : x ≡{n}≡ y → pcore x = some cx →
@@ -332,53 +269,13 @@ theorem pcore_ne {x y : GenSetO S} : x ≡{n}≡ y → pcore x = some cx →
   intro H1 H2
   exists y
   simp only [pcore, Option.some.injEq, true_and] at H2 ⊢
-  rw [<-H2]
+  rw [←H2]
   exact H1
-
-theorem validN_ne {x y : GenSetO S} : x ≡{n}≡ y → validN n x → validN n y := by
-  intro _ _; simp [validN, valid]
-
-theorem valid_iff_validN {x : GenSetO S} : valid x ↔ ∀ n, validN n x := by
-  simp [validN, valid]
-
-theorem validN_succ {x : GenSetO S} : validN n.succ x → validN n x := by
-  intro _; simp [validN, valid]
-
-theorem pcore_idem {x : GenSetO S} : pcore x = some cx → pcore cx ≡ some cx := by
-  simp [pcore]
-
-theorem pcore_unit : pcore (unit : GenSetO S) ≡ some unit := by
-  simp [pcore, unit]
 
 def op (x y : GenSetO S) : GenSetO S := gen_set_valid (x.car ∪ y.car)
 
-theorem validN_op_left {x y : GenSetO S} : validN n (op x y) → validN n x := by
-  intro _; simp [validN, valid]
-
 instance op_ne {x : GenSetO S} : OFE.NonExpansive (op x) where
-  ne n y z H := by simp [op]; rw [H]
-
-theorem assoc {x y z : GenSetO S} : op x (op y z) ≡ op (op x y) z := by
-  simp [op, union_assoc]
-
-theorem comm {x y : GenSetO S} : op x y ≡ op y x := by
-  simp [op, union_comm]
-
-theorem pcore_op_left {x : GenSetO S} : pcore x = some cx → op cx x ≡ x := by
-  simp only [pcore, Option.some.injEq, op, leibniz]
-  rintro ⟨⟩; simp [union_idem]
-
-theorem pcore_op_mono {x : GenSetO S} : pcore x = some cx → ∀ y, ∃ cy, pcore (op x y) ≡ some (op cx cy) := by
-  simp only [pcore, Option.some.injEq, leibniz]
-  rintro ⟨⟩ y
-  exists y
-
-def extend {x y₁ y₂ : GenSetO S} (H : x ≡{n}≡ op y₁ y₂) :
-    Σ' z₁ z₂, x ≡ op z₁ z₂ ∧ z₁ ≡{n}≡ y₁ ∧ z₂ ≡{n}≡ y₂ := by
-  exists y₁, y₂
-
-theorem unit_left_id {x : GenSetO S} : op unit x ≡ x := by
-  simp [op, unit, union_empty_left]
+  ne _ _ _ H := by simp only [op]; rw [H]
 
 instance : CMRA (GenSetO S) where
   pcore := pcore
@@ -387,22 +284,23 @@ instance : CMRA (GenSetO S) where
   Valid := valid
   op_ne := op_ne
   pcore_ne := pcore_ne
-  validN_ne := validN_ne
-  valid_iff_validN := valid_iff_validN
-  validN_succ := validN_succ
-  validN_op_left := validN_op_left
-  assoc := assoc
-  comm := comm
-  pcore_op_left := pcore_op_left
-  pcore_idem := pcore_idem
-  pcore_op_mono := pcore_op_mono
-  extend _ := extend
+  validN_ne := by intro _ _; simp [validN, valid]
+  valid_iff_validN := by simp [validN, valid]
+  validN_succ := by intro _; simp [validN, valid]
+  validN_op_left := by intro _; simp [validN, valid]
+  assoc := by simp [op, union_assoc]
+  comm := by simp [op, union_comm]
+  pcore_op_left {_ x} := by
+    simp only [pcore, Option.some.injEq, op, leibniz]; rintro ⟨⟩; simp [union_idem]
+  pcore_idem := by simp [pcore]
+  pcore_op_mono heq y := by simp only [pcore, Option.some.injEq] at heq; cases heq; exists y
+  extend {_ _ y₁ y₂} _ h := ⟨y₁, y₂, ⟨h, rfl, rfl⟩⟩
 
 instance : UCMRA (GenSetO S) where
   unit := unit
-  unit_valid := unit_valid
-  unit_left_id := unit_left_id
-  pcore_unit := pcore_unit
+  unit_valid := by simp [CMRA.Valid, valid]
+  unit_left_id := by simp [CMRA.op, op, unit, union_empty_left]
+  pcore_unit := by simp [CMRA.pcore, pcore, unit]
 
 theorem set_op (X Y : GenSetO S) : X • Y ≡ gen_set_valid (X.car ∪ Y.car) := by
   simp [CMRA.op, op]
@@ -414,16 +312,16 @@ theorem set_core (X : GenSetO S) : CMRA.core X ≡ X := by
 
 theorem set_included (X Y : S) : gen_set_valid X ≼ gen_set_valid Y ↔ X ⊆ Y := by
   simp only [CMRA.Included]
-  apply Iff.intro
+  constructor
   · intro ⟨Z, HZ⟩
-    simp [CMRA.op, op] at HZ
+    simp only [CMRA.op, op, leibniz, LeibnizO.mk.injEq] at HZ
     rw [HZ]
     intro p Hp; rw [mem_union]; left; exact Hp
   · intro Hsub
     exists gen_set_valid (Y \ X)
-    simp [CMRA.op, op]
+    simp only [CMRA.op, op, leibniz, LeibnizO.mk.injEq]
     ext p; rw [mem_union, mem_diff]
-    apply Iff.intro
+    constructor
     · intro G
       by_cases H : (p ∈ X)
       · left; exact H
